Add annotated version of inductive chain demo

demos/ch04/inductive_chain.dfy
@@ -1,4 +1,6 @@
 module Ex {
+  // This simple example illustrates what the process of looking for an
+  // inductive invariant might look like.
 
   datatype Variables = Variables(p1: bool, p2: bool, p3: bool, p4: bool)
 
@@ -9,11 +11,16 @@ module Ex {
     && !v.p4
   }
 
+  // The state machine starts out with all four booleans false, and it "turns
+  // on" p1, p2, p3, and p4 in order. The safety property says p4 ==> p1;
+  // proving this requires a stronger inductive invariant.
+
   datatype Step =
     | Step1
     | Step2
     | Step3
     | Step4
+    | Noop
 
   ghost predicate NextStep(v: Variables, v': Variables, step: Step)
   {
@@ -28,6 +35,7 @@ module Ex {
         v.p2 && v' == v.(p3 := true)
       case Step4 =>
         v.p3 && v' == v.(p4 := true)
+      case Noop => v' == v
     }
   }
 
@@ -43,19 +51,38 @@ module Ex {
 
   ghost predicate Inv(v: Variables)
   {
+    // SOLUTION
+    // This is one approach: prove implications that go all the way back to the
+    // beginning, trying to slowly work our way up to something inductive.
     && Safety(v)
+    && (v.p3 ==> v.p1)
+    && (v.p2 ==> v.p1)
+    // END
   }
 
   lemma InvInductive(v: Variables, v': Variables)
     requires Inv(v) && Next(v, v')
     ensures Inv(v')
   {
+    // SOLUTION
+    // This :| syntax is called "assign-such-that". Think of it as telling Dafny
+    // to assign step a value such that NextStep(v, v', step) (the predicate on
+    // the RHS) holds. What Dafny will do is first prove there exists such a
+    // step, then bind an arbitrary value to step where NextStep(v, v', step)
+    // holds for the remainder of the proof.
     var step :| NextStep(v, v', step);
+    assert NextStep(v, v', step); // by definition of :|
+    // END
     match step {
       case Step1 => { return; }
       case Step2 => { return; }
       case Step3 => { return; }
-      case Step4 => { return; }
+      case Step4 => {
+        // SOLUTION
+        return;
+        // END
+      }
+      case Noop => { return; }
     }
   }
 
@@ -65,6 +92,8 @@ module Ex {
     return;
   }
 
+  // This is the main inductive proof of Safety, but we moved all the difficult
+  // reasoning to the lemmas above.
   lemma SafetyHolds(v: Variables, v': Variables)
     ensures Init(v) ==> Inv(v)
     ensures Inv(v) && Next(v, v') ==> Inv(v')
@@ -75,4 +104,58 @@ module Ex {
     }
     InvSafe(v);
   }
+
+  // SOLUTION
+  // Instead of worrying about Safety, we can approach invariants by starting
+  // with properties that should hold in all reachable states. The advantage of
+  // this approach is that we can "checkpoint" our work of writing an invariant
+  // that characterizes reachable states. The disadvantage is that we might
+  // prove properties that don't help with safety and waste time.
+  //
+  // Recall that an invariant may have a counterexample to induction (CTI): a
+  // way to start in a state satisfying the invariant and transition out of it.
+  // If the invariant really holds, then a CTI simply reflects an unreachable
+  // state, one that we should try to eliminate by strengthening the invariant.
+  // If we find a "self-inductive" property Inv that satisfies Init(v) ==>
+  // Inv(v) and Inv(v) && Next(v, v') ==> Inv(v'), then we can extend it without
+  // fear of breaking inductiveness: in proving Inv(v) && Inv2(v) && Next(v, v')
+  // ==> Inv(v') && Inv2(v'), notice that we can immediately prove Inv(v').
+  // However, we've also made progress: in proving Inv2(v'), we get to know
+  // Inv(v). This may rule out some CTIs, and eventually will be enough to prove
+  // Inv2 is inductive.
+  //
+  // Notice that the above discussion involved identifying a self-inductive
+  // invariant without trying to prove a safety property. This is one way to go
+  // about proving safety: start by proving "easy" properties that hold in
+  // reachable states. This will reduce the burden of getting CTIs (or failed
+  // proofs). However, don't spend all your time proving properties about
+  // reachable states: there will likely be properties that really are
+  // invariants, but (a) the proof is complicated and (b) they don't help you
+  // prove safety.
+
+  predicate Inv2(v: Variables) {
+    // each of these conjuncts is individually "self-inductive", but all of them
+    // are needed together to actually prove safety
+    && (v.p2 ==> v.p1)
+    && (v.p3 ==> v.p2)
+    && (v.p4 ==> v.p3)
+  }
+
+  lemma Inv2Holds(v: Variables, v': Variables)
+    ensures Init(v) ==> Inv(v)
+    ensures Inv(v) && Next(v, v') ==> Inv(v')
+  {
+    assert Init(v) ==> Inv(v);
+    if Inv(v) && Next(v, v') {
+      var step :| NextStep(v, v', step);
+      match step {
+        case Step1 => { return; }
+        case Step2 => { return; }
+        case Step3 => { return; }
+        case Step4 => { return; }
+        case Noop => { return; }
+      }
+    }
+  }
+  // END
 }
